Refactor `RankAxioms.lean`

Matroid/Constructions/RankAxioms.lean
@@ -1,5 +1,6 @@
 import Mathlib.Data.Matroid.Basic
 import Mathlib.Data.Matroid.IndepAxioms
+import Matroid.Minor.Rank
 
 /-- A matroid as defined by the (relative) rank axioms. The constructed
   `RankMatroid` can be then converted into a `Matroid` with `RankMatroid.matroid` -/
@@ -8,21 +9,24 @@ structure RankMatroid (α : Type*) where
   (E : Set α)
   /-- The (relative) rank function -/
   (relRank : Set α → Set α → ℕ∞)
+  (relRank_le_encard_diff (A B : Set α) : relRank A B ≤ (B \ A).encard)
+  (relRank_union_le_relRank_inter (A B : Set α) : relRank B (A ∪ B) ≤ relRank (A ∩ B) A)
+  (relRank_add_cancel {A B C : Set α} : A ⊆ B → B ⊆ C → relRank A C = relRank A B + relRank B C)
+  (relRank_sUnion_eq_zero {S : Set (Set α)} {A : Set α} :
+      (∀ B ∈ S, A ⊆ B ∧ relRank A B = 0) → relRank A (⋃₀ S) = 0)
 
-  (rel_rank_le_encard_diff {A B : Set α} : A ⊆ E → B ⊆ A → relRank A B ≤ (A \ B).encard)
-  (rel_rank_union_le_relRank_inter {A B : Set α} : A ⊆ E → B ⊆ E →
-    relRank (A ∪ B) B ≤ relRank A (A ∩ B))
-  (rel_rank_add_cancel {A B C : Set α} : A ⊆ E → B ⊆ A → C ⊆ B → (relRank A C) = (relRank A B) + (relRank B C))
-  (rel_rank_sUnion_eq_zero {S : Set (Set α)} {B : Set α} :
-      (∀ A ∈ S, B ⊆ A ∧ A ⊆ E ∧ relRank A B = 0) → relRank (⋃₀ S) B = 0)
+  -- do we need both inter_ground_left and inter_ground_right?
+  (relRank_inter_ground_left (A B : Set α) : relRank (A ∩ E) B = relRank A B)
+  (relRank_inter_ground_right (A B : Set α) : relRank A (B ∩ E) = relRank A B)
+  (relRank_eq_union_right (A B : Set α) : relRank A B = relRank A (B ∪ A))
 
   (Indep : Set α → Prop)
   (indep_maximal : ∀ X ⊆ E, Matroid.ExistsMaximalSubsetProperty Indep X)
-  (indep_iff' : ∀ I, Indep I ↔ I ⊆ E ∧ ∀ x ∈ I, relRank I (I \ {x}) > 0 )
+  (indep_iff' {I : Set α} : Indep I ↔ I ⊆ E ∧ ∀ x ∈ I, relRank (I \ {x}) I > 0 )
 
 namespace RankMatroid
 
-variable {α : Type*} {A B I J X : Set α} {M : RankMatroid α} {x : α}
+variable {α : Type*} {A B I J X : Set α} {x : α}
 
 def indepSubsets (M : RankMatroid α) (A : Set α) : Set (Set α) :=
   {I | M.Indep I ∧ I ⊆ A}
@@ -30,33 +34,31 @@ def indepSubsets (M : RankMatroid α) (A : Set α) : Set (Set α) :=
 def Basis' (M : RankMatroid α) (I A : Set α) : Prop :=
   I ∈ maximals (· ⊆ ·) (M.indepSubsets A)
 
-theorem r_nonneg : M.relRank A B ≥ 0 := by
-  exact zero_le (M.relRank A B)
+lemma relRank_self_eq_zero {M : RankMatroid α} : M.relRank A A = 0 := by
+  obtain h := M.relRank_le_encard_diff A A
+  simpa only [sdiff_self, Set.bot_eq_empty, Set.encard_empty, nonpos_iff_eq_zero] using h
 
-theorem relRank_self_eq_zero (h : A ⊆ M.E) : M.relRank A A = 0 := by
-  have := M.rel_rank_le_encard_diff h (subset_refl A)
-  rw [Set.diff_eq_empty.mpr fun ⦃a⦄ a ↦ a, Set.encard_empty] at this
-  exact nonpos_iff_eq_zero.mp this
+lemma Indep.subset_ground {M : RankMatroid α} (h : M.Indep I) : I ⊆ M.E :=
+  (M.indep_iff'.mp h).left
 
-theorem Indep.subset_ground (h : M.Indep I) : I ⊆ M.E := by
-  rw [indep_iff'] at h
-  exact h.left
+lemma Indep.indep {M : RankMatroid α} (h : M.Indep I) : ∀ x ∈ I, M.relRank (I \ {x}) I > 0 :=
+  (M.indep_iff'.mp h).right
 
-theorem Indep.indep (h : M.Indep I) :  ∀ x ∈ I, M.relRank I (I \ {x}) > 0  := by
-  rw [indep_iff'] at h
-  exact h.right
+lemma Indep.relRank_pos_of_sub_mem {M : RankMatroid α} (h : M.Indep I) (hx : x ∈ I) :
+    M.relRank (I \ {x}) I > 0 :=
+  h.indep x hx
 
-theorem indep_subset (hJ : M.Indep J) (rIJ : I ⊆ J) : M.Indep I := by
-  rw [M.indep_iff']
-  refine ⟨rIJ.trans hJ.subset_ground, fun x hx ↦ ?_⟩
-  have hJ_indep := hJ.subset_ground
-  have hJ := hJ.indep x (Set.mem_of_mem_of_subset hx rIJ)
+lemma relRank_inter_ground {M : RankMatroid α} : M.relRank (A ∩ M.E) (B ∩ M.E) = M.relRank A B := by
+  rw [M.relRank_inter_ground_left, M.relRank_inter_ground_right]
+
+lemma indep_subset {M : RankMatroid α} (hJ : M.Indep J) (rIJ : I ⊆ J) : M.Indep I := by
+  refine M.indep_iff'.mpr ⟨rIJ.trans hJ.subset_ground, fun x hx ↦ ?_⟩
+  have hJ := hJ.relRank_pos_of_sub_mem (rIJ hx)
   set A := I
   set B := J \ {x}
-  have hAUB : J = A ∪ B := by
-    refine (Set.union_diff_cancel' ?h₁ rIJ).symm
-    exact Set.singleton_subset_iff.mpr hx
-  have hAIB : A \ {x} = A ∩ B := by
+  have hAUB : J = I ∪ (J \ {x}) :=
+    (Set.union_diff_cancel' (Set.singleton_subset_iff.mpr hx) rIJ).symm
+  have hAIB : I \ {x} = I ∩ (J \ {x}) := by
     ext y;
     refine ⟨fun hY ↦ ?_, fun hY ↦ ?_⟩
     · refine ⟨Set.mem_of_mem_diff hY, Set.mem_diff_singleton.mpr ?_⟩
@@ -68,21 +70,21 @@ theorem indep_subset (hJ : M.Indep J) (rIJ : I ⊆ J) : M.Indep I := by
     exact ⟨Set.mem_of_mem_inter_left hY, hynex⟩
   rw [hAUB] at hJ
   rw [hAIB]
-  have hA : A ⊆ M.E := (rIJ.trans hJ_indep)
-  have hB : B ⊆ M.E := ((Set.diff_subset).trans hJ_indep)
-  exact hJ.trans_le (M.rel_rank_union_le_relRank_inter hA hB)
+  exact hJ.trans_le (M.relRank_union_le_relRank_inter A B)
 
-theorem r_le_r_subset_right (hX : X ⊆ M.E) (hAX : A ⊆ X) (hBA : B ⊆ A) : M.relRank X A ≤ M.relRank X B := by
-  rw [M.rel_rank_add_cancel hX hAX hBA]; simp only [self_le_add_right]
+lemma relRank_mono_left {M : RankMatroid α} (hBX : B ⊆ X) (hAB : A ⊆ B) :
+    M.relRank B X ≤ M.relRank A X := by
+  rw [M.relRank_add_cancel hAB hBX]
+  simp only [self_le_add_left]
 
-theorem insert_indep_iff_r_insert_pos (hI_indep : M.Indep I) (hx : x ∈ M.E \ I)
-    : M.Indep (Set.insert x I) ↔ M.relRank (Set.insert x I) I > 0 := by
+lemma insert_indep_iff_relRank_insert_pos {M : RankMatroid α} (hI_indep : M.Indep I)
+    (hx : x ∈ M.E \ I) : M.Indep (Set.insert x I) ↔ M.relRank I (Set.insert x I) > 0 := by
   refine ⟨fun hIx_indep ↦ ?_, fun hr ↦ ?_⟩
   · have h := hIx_indep.indep x (Set.mem_insert x I)
     have : Set.insert x I \ {x} = I :=
       Set.insert_diff_self_of_not_mem (Set.not_mem_of_mem_diff hx)
     rwa [this] at h
-  refine (M.indep_iff' (Set.insert x I)).mpr ?_
+  refine M.indep_iff'.mpr ?_
   refine ⟨Set.insert_subset (Set.mem_of_mem_diff hx) hI_indep.subset_ground, ?_⟩
   contrapose! hr
   rcases hr with ⟨y, hy, hr⟩
@@ -91,18 +93,18 @@ theorem insert_indep_iff_r_insert_pos (hI_indep : M.Indep I) (hx : x ∈ M.E \ I
     have := Set.not_mem_of_mem_diff hx
     have : Set.insert y I \ {y} = I := Set.insert_diff_self_of_not_mem this
     rwa [this] at hr
-  have h : M.relRank (Set.insert x I) (I \ {y}) ≤ 1 := by
-    set A := (Set.insert x I)
+  have h : M.relRank (I \ {y}) (Set.insert x I) ≤ 1 := by
+    set C := (Set.insert x I)
     set B := (Set.insert x I \ {y})
-    set C := (I \ {y})
-    have h₁ : A ⊆ M.E := Set.insert_subset (Set.mem_of_mem_diff hx) hI_indep.subset_ground
-    have h₂ : B ⊆ A := @Set.diff_subset α (insert x I) {y}
-    have h₃ : C ⊆ B := by
+    set A := (I \ {y})
+    have h₁ : C ⊆ M.E := Set.insert_subset (Set.mem_of_mem_diff hx) hI_indep.subset_ground
+    have h₂ : B ⊆ C := @Set.diff_subset α (insert x I) {y}
+    have h₃ : A ⊆ B := by
       refine Set.diff_singleton_subset_iff.mpr ?_
       rw [Set.insert_diff_singleton]
       exact (Set.subset_insert x I).trans (Set.subset_insert y (Set.insert x I))
-    have hrBC : M.relRank B C ≤ 1 := by
-      have h := M.rel_rank_le_encard_diff (h₂.trans h₁) h₃
+    have hrAB : M.relRank A B ≤ 1 := by
+      have h := M.relRank_le_encard_diff A B
       rw [Set.diff_diff_right] at h
       have h := h.trans (Set.encard_union_le (B \ I) (B ∩ {y}))
       rw [Set.encard_eq_zero.mpr Set.diff_inter_self] at h
@@ -112,18 +114,18 @@ theorem insert_indep_iff_r_insert_pos (hI_indep : M.Indep I) (hx : x ∈ M.E \ I
       · rw [h'] at h; rw [Set.encard_empty] at h; exact h.trans zero_le_one
       rw [h'] at h; rwa [Set.encard_singleton] at h;
     have h : M.relRank A B + M.relRank B C <= 1 := by
-      exact add_le_add hr hrBC
-    have := M.rel_rank_add_cancel h₁ h₂ h₃
+      exact add_le_add hrAB hr
+    have := M.relRank_add_cancel h₃ h₂
     rwa [<-this] at h
-  set A := (Set.insert x I)
+  set C := (Set.insert x I)
   set B := (I)
-  set C := (I \ {y})
+  set A := (I \ {y})
   have h' : M.relRank A C = M.relRank A B + M.relRank B C := by
-    have h₁ : A ⊆ M.E := Set.insert_subset (Set.mem_of_mem_diff hx) hI_indep.subset_ground
-    have h₂ : B ⊆ A := Set.subset_insert x I
-    have h₃ : C ⊆ B := Set.diff_subset
-    exact M.rel_rank_add_cancel h₁ h₂ h₃
-  have h'' : M.relRank B C ≥ 1 := by
+    have h₁ : C ⊆ M.E := Set.insert_subset (Set.mem_of_mem_diff hx) hI_indep.subset_ground
+    have h₂ : B ⊆ C := Set.subset_insert x I
+    have h₃ : A ⊆ B := Set.diff_subset
+    exact M.relRank_add_cancel h₃ h₂
+  have h'' : M.relRank A B ≥ 1 := by
     rcases Set.mem_insert_iff.mp hy with rfl | hy
     · contradiction
     have := hI_indep.indep y hy
@@ -132,31 +134,34 @@ theorem insert_indep_iff_r_insert_pos (hI_indep : M.Indep I) (hx : x ∈ M.E \ I
   rw [h'];
   have h := ENat.add_one_le_of_lt h
   simp only [zero_add] at h
-  have := add_le_add h h''
+  have := add_le_add h'' h
   rw [one_add_one_eq_two] at this
   refine (ENat.add_one_le_iff ?refine_2.intro.intro.hm).mp this
   exact ENat.coe_toNat_eq_self.mp rfl
 
-theorem indep_subset_maximal_iff_relrank_zero (hX : X ⊆ M.E) (hI : I ⊆ X) (hI_indep : M.Indep I) :
-    (I ∈ (maximals (· ⊆ ·) {S | M.Indep S ∧ S ⊆ X}) ↔ M.relRank X I = 0) := by
+lemma indep_subset_maximal_iff_relRank_zero {M : RankMatroid α} (hI : I ⊆ X) (hI_indep : M.Indep I) :
+    (I ∈ (maximals (· ⊆ ·) {S | M.Indep S ∧ S ⊆ X}) ↔ M.relRank I X = 0) := by
   refine ⟨fun hI_max ↦ ?_, fun hr ↦ ?_⟩
   · by_cases hXI : X = I
-    · rw [hXI]; exact relRank_self_eq_zero hI_indep.subset_ground
+    · rw [hXI]; exact relRank_self_eq_zero
     set S := {(insert x I) | x ∈ X \ I}
-    have h : ∀ A ∈ S, I ⊆ A ∧ A ⊆ M.E ∧ M.relRank A I = 0 := by
+    have h : ∀ A ∈ S, I ⊆ A ∧ M.relRank I A = 0 := by
       rintro A ⟨x, hx_mem, rfl⟩
+      refine ⟨Set.subset_insert x I, ?_⟩
       rcases (Set.mem_diff x).mpr hx_mem with ⟨hxX, hxI⟩
-      refine ⟨Set.subset_insert x I, Set.insert_subset (hX hxX) hI_indep.subset_ground, ?_⟩
+      by_cases hx : x ∉ M.E
+      · rw [<-M.relRank_inter_ground, Set.insert_inter_of_not_mem hx, M.relRank_self_eq_zero]
+      simp only [not_not] at hx
       contrapose! hI_max
-      have hI_max : M.relRank (insert x I) I > 0 := by exact pos_iff_ne_zero.mpr hI_max
+      have hI_max : M.relRank I (insert x I) > 0 := by exact pos_iff_ne_zero.mpr hI_max
       suffices h : M.Indep (insert x I) by
         have : (insert x I) ∈ {S | M.Indep S ∧ S ⊆ X} := ⟨h, Set.insert_subset hxX hI⟩
         apply mem_maximals_iff.not.mpr
         push_neg; intro; use (insert x I)
         exact ⟨this, Set.subset_insert x I, by exact Set.ne_insert_of_not_mem I hxI⟩
-      have hxEI : x ∈ M.E \ I := by exact (Set.mem_diff x).mpr ⟨hX hxX, hxI⟩
-      exact (insert_indep_iff_r_insert_pos hI_indep hxEI).mpr hI_max
-    have := M.rel_rank_sUnion_eq_zero h
+      have hxEI : x ∈ M.E \ I := by exact (Set.mem_diff x).mpr ⟨hx, hxI⟩
+      exact (insert_indep_iff_relRank_insert_pos hI_indep hxEI).mpr hI_max
+    have := M.relRank_sUnion_eq_zero h
     have hXU : X = S.sUnion := by
       apply Set.eq_of_subset_of_subset
       · intro x hx; simp only [Set.mem_sUnion]
@@ -184,14 +189,14 @@ theorem indep_subset_maximal_iff_relrank_zero (hX : X ⊆ M.E) (hI : I ⊆ X) (h
   obtain ⟨x, hxI', hxI⟩ := Set.exists_of_ssubset hI'_ssubset
   have : M.Indep (Set.insert x I) := by
     exact indep_subset hI'_indep (Set.insert_subset hxI' hI'_ssubset.subset)
-  rw [insert_indep_iff_r_insert_pos hI_indep ((Set.mem_diff x).mpr ⟨(hI'.trans hX) hxI', hxI⟩)] at this
-  have : M.relRank X I > 0 := by
-    rw [M.rel_rank_add_cancel hX (Set.insert_subset (hI' hxI') hI) (Set.subset_insert x I)]
-    have this' : M.relRank X (Set.insert x I) ≥ 0 := by exact r_nonneg
-    exact Right.add_pos_of_nonneg_of_pos this' this
+  have hx : x ∈ M.E := hI'_indep.subset_ground hxI'
+  rw [insert_indep_iff_relRank_insert_pos hI_indep ((Set.mem_diff x).mpr ⟨hx, hxI⟩)] at this
+  have : M.relRank I X > 0 := by
+    rw [M.relRank_add_cancel (Set.subset_insert x I) (Set.insert_subset (hI' hxI') hI)]
+    exact Left.add_pos_of_pos_of_nonneg this (zero_le (M.relRank (Set.insert x I) X))
   exact pos_iff_ne_zero.mp this
 
-@[simps] protected def indepMatroid (M : RankMatroid α) : IndepMatroid α where
+@[simps!] protected def indepMatroid (M : RankMatroid α) : IndepMatroid α where
   E := M.E
   Indep := M.Indep
 
@@ -212,38 +217,39 @@ theorem indep_subset_maximal_iff_relrank_zero (hX : X ⊆ M.E) (hI : I ⊆ X) (h
 
     intro I B hI_indep hI_nmax hB_max
     have hB_indep := (mem_maximals_iff.mp hB_max).left
-    have hrEI : M.relRank M.E I > 0 := by
+    have hrIE : M.relRank I M.E > 0 := by
       contrapose! hI_nmax
       norm_num at hI_nmax
-      have := (indep_subset_maximal_iff_relrank_zero (subset_refl M.E) hI_indep.subset_ground hI_indep).mpr
+      have := (indep_subset_maximal_iff_relRank_zero hI_indep.subset_ground hI_indep).mpr
       rw [hiff] at this
       exact this hI_nmax
-    have hrEB : M.relRank M.E B = 0 := by
-      have := (indep_subset_maximal_iff_relrank_zero (subset_refl M.E) hB_indep.subset_ground hB_indep).mp
+    have hrBE : M.relRank B M.E = 0 := by
+      have := (indep_subset_maximal_iff_relRank_zero hB_indep.subset_ground hB_indep).mp
       rw [hiff] at this
       exact this hB_max
-    have hrIUB_I : M.relRank (I ∪ B) I > 0 := by
+    have hrI_IUB : M.relRank I (I ∪ B) > 0 := by
       have h₁ : I ⊆ (I ∪ B) := by exact Set.subset_union_left
       have h₂ : (I ∪ B) ⊆ M.E := by exact Set.union_subset hI_indep.subset_ground hB_indep.subset_ground
       have h₃ : M.E ⊆ M.E := by exact fun ⦃a⦄ a ↦ a
       calc
-      0 < M.relRank M.E I := by assumption
-      _ = M.relRank M.E (I ∪ B) + M.relRank (I ∪ B) I := by
-        exact M.rel_rank_add_cancel h₃ h₂ h₁
-      _ ≤ M.relRank M.E B + M.relRank (I ∪ B) I := by
-        apply add_le_add_right
-        exact r_le_r_subset_right h₃ h₂ (Set.subset_union_right)
-      _ = M.relRank (I ∪ B) I := by
-        rw [hrEB]
-        simp only [zero_add]
+      0 < M.relRank I M.E := by assumption
+      _ = M.relRank I (I ∪ B) + M.relRank (I ∪ B) M.E := by
+        exact M.relRank_add_cancel h₁ h₂
+      _ ≤ M.relRank I (I ∪ B) + M.relRank B M.E := by
+        apply add_le_add_left
+        exact relRank_mono_left h₂ (Set.subset_union_right)
+      _ = M.relRank I (I ∪ B) := by
+        rw [hrBE]
+        simp only [add_zero]
     have hIUB_subset := (Set.union_subset hI_indep.subset_ground hB_indep.subset_ground)
-    have hI_nmax := (not_iff_not.mpr (indep_subset_maximal_iff_relrank_zero hIUB_subset (Set.subset_union_left) hI_indep)).mpr (Ne.symm (hrIUB_I.ne))
+    have hI_nmax := (not_iff_not.mpr (indep_subset_maximal_iff_relRank_zero Set.subset_union_left hI_indep)).mpr (Ne.symm (hrI_IUB.ne))
     have h_maximals_nonempty := M.indep_maximal (I ∪ B) hIUB_subset I hI_indep  (Set.subset_union_left)
     rcases h_maximals_nonempty with ⟨I', ⟨hI'_indep, hI'_contains_I, hI'_in_IUB⟩, hI'_max⟩
     by_cases hII' : I = I'
     · rw [<-hII'] at hI'_max hI'_indep
       simp only [Set.mem_setOf_eq, and_imp] at hI'_max
       contrapose! hI_nmax
+      clear hI_nmax
       rw [mem_maximals_iff]; simp only [Set.mem_setOf_eq, Set.subset_union_left, and_true, and_imp]
       refine ⟨by assumption, ?_⟩
       intro y hy_indep hy_in hy_within
@@ -271,52 +277,38 @@ namespace Matroid
 
 variable {α : Type*} {I : Set α}
 
-def indepSubsets (M : Matroid α) (A : Set α) : Set (Set α) :=
-  {I | M.Indep I ∧ I ⊆ A}
+-- def indepSubsets (M : Matroid α) (A : Set α) : Set (Set α) :=
+--   {I | M.Indep I ∧ I ⊆ A}
 
-noncomputable def relRank (M : Matroid α) (A B : Set α) : ℕ∞ :=
-  sSup {x | ∃ I J : Set α, J ⊆ I ∧ I ∈ M.indepSubsets A ∧ M.Basis' J B ∧ x = (I \ J).encard}
+-- noncomputable def relRank (M : Matroid α) (A B : Set α) : ℕ∞ :=
+--   sSup {x | ∃ I J : Set α, J ⊆ I ∧ I ∈ M.indepSubsets A ∧ M.Basis' J B ∧ x = (I \ J).encard}
 
-theorem basis_of_maximal_extension (M : Matroid α) {I X J : Set α}
-    (h : J ∈ maximals (· ⊆ ·) {I' | M.Indep I' ∧ I ⊆ I' ∧ I' ⊆ X}) : M.Basis' J X := by
-  unfold Basis'; unfold maximals at h ⊢; simp only [Set.mem_setOf_eq, and_imp] at h ⊢
+lemma basis_of_maximal_extension (M : Matroid α) {I X J : Set α}
+    (hX : X ⊆ M.E) (h : J ∈ maximals (· ⊆ ·) {I' | M.Indep I' ∧ I ⊆ I' ∧ I' ⊆ X}) : M.Basis J X := by
+  unfold Basis; unfold maximals at h ⊢; simp only [Set.mem_setOf_eq, and_imp] at h ⊢
   obtain ⟨⟨hJ_indep, hIJ, hJX⟩, hJ_max⟩ := h
-  refine ⟨⟨hJ_indep, hJX⟩, ?_⟩
+  refine ⟨⟨⟨hJ_indep, hJX⟩, ?_⟩, hX⟩
   intro J' hJ'_indep hJ'X hJJ'
   exact hJ_max hJ'_indep (hIJ.trans hJJ') hJ'X hJJ'
 
-theorem rel_rank_eq_any_choice (M : Matroid α) {A B : Set α} (hB : B ⊆ A) (hA : A ⊆ M.E) {I J : Set α}
-    (h : J ⊆ I) (hI : M.Basis' I A) (hJ : M.Basis' J B) :
-    M.relRank A B = (I \ J).encard := by
-  unfold Basis' maximals at hJ; simp only [Set.mem_setOf_eq, and_imp] at hJ
-  have ⟨⟨hJ_indep, hJ_subset_B⟩, hJ_max⟩ := hJ
-  apply le_antisymm_iff.mpr; rw [and_comm]
-  constructor
-  · have : (I \ J).encard ∈ {x | ∃ I J : Set α, J ⊆ I ∧ I ∈ M.indepSubsets A ∧ J ∈ maximals (· ⊆ ·) (M.indepSubsets B) ∧ x = (I \ J).encard} := by
-      use I, J; unfold maximals indepSubsets; simp only [Set.mem_setOf_eq, and_imp, and_true];
-      unfold Basis' at hI
-      exact ⟨h, (maximals_subset (fun a b ↦ a ⊆ b) (M.indepSubsets A)) hI, hJ.1, hJ.2⟩
-    exact le_sSup this
-  apply sSup_le; intro r; simp only [Set.mem_setOf_eq, forall_exists_index, and_imp]
-  rintro I' J' h' hI' hJ' rfl
-  sorry
-
-theorem rel_rank_exists (M : Matroid α) {A B : Set α} (hB : B ⊆ A) (hA : A ⊆ M.E) :
-    ∃ I J : Set α, J ⊆ I ∧ M.Basis' I A ∧ M.Basis' J B ∧ M.relRank A B = (I \ J).encard := by
-  obtain ⟨J, hJ⟩ := M.maximality B (hB.trans hA) ∅ M.empty_indep (Set.empty_subset B)
-  unfold maximals at hJ; simp only [Set.empty_subset, true_and, Set.mem_setOf_eq, and_imp] at hJ
-  have ⟨⟨hJ_indep, hJ_subset_B⟩, hJ_max⟩ := hJ
-  obtain ⟨I, hI⟩ := M.maximality A hA J hJ_indep (hJ_subset_B.trans hB)
+lemma relRank_intro (M : Matroid α) {A B : Set α} (hA : A ⊆ B) (hB : B ⊆ M.E) :
+    ∃ I J : Set α, I ⊆ J ∧ M.Basis I A ∧ M.Basis J B ∧ M.relRank A B = (J \ I).encard := by
+  -- sorry
+  obtain ⟨I, hI⟩ := M.maximality A (hA.trans hB) ∅ M.empty_indep (Set.empty_subset A)
+  unfold maximals at hI; simp only [Set.empty_subset, true_and, Set.mem_setOf_eq, and_imp] at hI
+  have ⟨⟨hI_indep, hI_subset_A⟩, _⟩ := hI
+  obtain ⟨J, hJ⟩ := M.maximality B hB I hI_indep (hI_subset_A.trans hA)
   use I; use J
-  unfold Basis'
-  have hIJ : J ⊆ I := hI.1.2.1
-  have hI_basis : M.Basis' I A := by
-    refine M.basis_of_maximal_extension hA (hJ.1.2.trans hB) hJ.1.1 hI
-  have hJ_basis : M.Basis' J B := by
-    refine M.basis_of_maximal_extension (hB.trans hA) (Set.empty_subset B) M.empty_indep ?_
+  unfold Basis
+  have hIJ : I ⊆ J := hJ.1.2.1
+  have hI_basis : M.Basis I A := by
+    refine @basis_of_maximal_extension α M ∅ A I (hA.trans hB) ?_
     unfold maximals; simp only [Set.empty_subset, true_and, Set.mem_setOf_eq, and_imp]
     assumption
-  exact ⟨hIJ, hI_basis, hJ_basis, M.rel_rank_eq_any_choice hB hA hIJ hI_basis hJ_basis⟩
+  have hJ_basis : M.Basis J B := by
+    refine M.basis_of_maximal_extension hB hJ
+  refine ⟨hIJ, hI_basis, hJ_basis, ?_⟩
+  exact Basis.relRank_eq_encard_diff_of_subset_basis hI_basis hJ_basis hIJ
 
 end Matroid
 
@@ -324,45 +316,44 @@ namespace RankMatroid
 
 variable {α : Type*} {A B I J X : Set α} {M : RankMatroid α} {x : α}
 
-theorem relRank_indeps_eq_encard_diff (M : RankMatroid α) {A B : Set α} (hB : B ⊆ A)
-    (hA : M.Indep A) : M.relRank A B = (A \ B).encard := by
-  set P := fun n ↦ ∀ (A B : Set α), B ⊆ A → M.Indep A → (A \ B).encard = n → M.relRank A B = n
+lemma relRank_indeps_eq_encard_diff (M : RankMatroid α) {A B : Set α} (hA : A ⊆ B) (hB : M.Indep B)
+    : M.relRank A B = (B \ A).encard := by
+  set P := fun n ↦ ∀ (A B : Set α), A ⊆ B → M.Indep B → (B \ A).encard = n → M.relRank A B = n
   have h_induc : ∀ n : ℕ∞, P n := by
     intro n
     refine (@ENat.nat_induction P n ?_ ?_ ?_)
-    · intro A B hB hA_indep h
-      have := M.rel_rank_le_encard_diff hA_indep.subset_ground hB
+    · intro A B hA hB_indep h
+      have := M.relRank_le_encard_diff A B
       rw [h] at this; simp only [nonpos_iff_eq_zero] at this; assumption
-    · intro n hPn A B hB hA_indep h
+    · intro n hPn A B hA hB_indep h
       have : (n.succ : ℕ∞) > 0 := by exact NeZero.pos (n.succ : ℕ∞)
       rw [<-h] at this
       rcases (Set.encard_pos.mp this) with ⟨x, hx⟩
-      set A' := A \ {x}
-      have hxA : x ∈ A := Set.mem_of_mem_diff hx
-      have hAA' : A' ⊆ A := by exact Set.diff_subset
-      have hBA' : B ⊆ A' := Set.subset_diff_singleton hB (Set.not_mem_of_mem_diff hx)
-      have hA'_indep : M.Indep A' := M.indep_subset hA_indep hAA'
-      have hA'dB: A' \ B = (A \ B) \ {x} := by exact Set.diff_diff_comm
-      have : (A' \ B).encard = n := by
-        rw [hA'dB]
+      set B' := B \ {x}
+      have hxB : x ∈ B := Set.mem_of_mem_diff hx
+      have hB'B : B' ⊆ B := by exact Set.diff_subset
+      have hAB' : A ⊆ B' := Set.subset_diff_singleton hA (Set.not_mem_of_mem_diff hx)
+      have hB'_indep : M.Indep B' := M.indep_subset hB_indep hB'B
+      have hB'dA : B' \ A = (B \ A) \ {x} := by exact Set.diff_diff_comm
+      have : (B' \ A).encard = n := by
+        rw [hB'dA]
         rw [<-Set.encard_diff_singleton_add_one hx] at h
         simp only [Nat.succ_eq_add_one, Nat.cast_add, Nat.cast_one] at h
         exact WithTop.add_right_cancel (ENat.coe_toNat_eq_self.mp (refl 1)) h
-      have hrA'B : M.relRank A' B = n := hPn A' B hBA' hA'_indep this
-      have hrAA' : M.relRank A A' = 1 := by
-        have hle : M.relRank A A' <= 1 := by
-          have := M.rel_rank_le_encard_diff hA_indep.subset_ground (@Set.diff_subset α A {x})
-          rw [Set.diff_diff_cancel_left (Set.singleton_subset_iff.mpr hxA)] at this
+      have hrAB' : M.relRank A B' = n := hPn A B' hAB' hB'_indep this
+      have hrB'B : M.relRank B' B = 1 := by
+        have hle : M.relRank B' B <= 1 := by
+          have := M.relRank_le_encard_diff (B \ {x}) B
+          rw [Set.diff_diff_cancel_left (Set.singleton_subset_iff.mpr hxB)] at this
           simp only [Set.encard_singleton] at this; exact this
-        have hgt : M.relRank A A' > 0 := by exact hA_indep.indep x hxA
+        have hgt : M.relRank B' B > 0 := by exact hB_indep.indep x hxB
         refine le_antisymm_iff.mpr ⟨hle, ENat.one_le_iff_pos.mpr hgt⟩
-      rw [M.rel_rank_add_cancel hA_indep.subset_ground hAA' hBA', hrA'B, hrAA']
+      rw [M.relRank_add_cancel hAB' hB'B, hrAB', hrB'B]
       have h11: (1 : ℕ) = (1 : ℕ∞) := rfl
-      rw [<-h11, <-(ENat.coe_add 1 n), add_comm, Nat.succ_eq_add_one];
+      rw [<-h11, <-(ENat.coe_add n 1), Nat.succ_eq_add_one]
     intro hP A B hB hA_indep h
     by_contra! h_finite
-    have : ∃ n, M.relRank A B = n := by
-      exact exists_eq'
+    have : ∃ n, M.relRank A B = n := exists_eq'
     -- rcases Option.ne_none_iff_exists'.mp h_finite with ⟨c, hc⟩
     rcases this with ⟨c, hc⟩
     simp at h
@@ -374,184 +365,194 @@ theorem relRank_indeps_eq_encard_diff (M : RankMatroid α) {A B : Set α} (hB : 
       have : D.encard = (D.ncard : ℕ∞) := by exact Eq.symm (Set.Finite.cast_ncard_eq hD_finite)
       rw [this, congrArg (Nat.cast) hD_ncard, hcc]
     clear hD_ncard hD_finite h_finite
-    let B' := B ∪ D
-    have hD_subset_A : D ⊆ A := hD_subset.trans (Set.diff_subset)
-    have hB'_subset_A : B' ⊆ A := by exact (Set.union_subset hB hD_subset_A)
-    have hB'_indep : M.Indep B' := by exact M.indep_subset hA_indep hB'_subset_A
-    have hB'B : (B' \ B).encard = ↑(ENat.toNat c + 1) := by
-      have : B ∩ D ⊆ ∅ := by
-        have : Disjoint B (A \ B) := Set.disjoint_sdiff_right
-        have : Disjoint B D := by exact Set.disjoint_of_subset (fun ⦃a⦄ a ↦ a) hD_subset this
+    let A' := A ∪ D
+    have hD_subset_B : D ⊆ B := hD_subset.trans (Set.diff_subset)
+    have hA'_subset_B : A' ⊆ B := by exact (Set.union_subset hB hD_subset_B)
+    have hA'_indep : M.Indep A' := by exact M.indep_subset hA_indep hA'_subset_B
+    have hA'A : (A' \ A).encard = ↑(ENat.toNat c + 1) := by
+      have : A ∩ D ⊆ ∅ := by
+        have : Disjoint A (B \ A) := Set.disjoint_sdiff_right
+        have : Disjoint A D := by exact Set.disjoint_of_subset (fun ⦃a⦄ a ↦ a) hD_subset this
         exact Set.disjoint_iff.mp this
       rw [Set.union_diff_cancel_left this, hD_encard, hcc]
-    have hrB'B : M.relRank B' B = c + 1 := by
-      rw [hP (ENat.toNat c + 1) B' B (Set.subset_union_left) hB'_indep hB'B, hcc]
+    have hrAA' : M.relRank A A' = c + 1 := by
+      rw [hP (ENat.toNat c + 1) A A' (Set.subset_union_left) hA'_indep hA'A, hcc]
     have hbad : M.relRank A B ≥ c + 1 := by
-      rw [M.rel_rank_add_cancel hA_indep.subset_ground hB'_subset_A (Set.subset_union_left), hrB'B]
-      simp only [ge_iff_le, self_le_add_left]
+      rw [M.relRank_add_cancel Set.subset_union_left hA'_subset_B, hrAA']
+      simp only [ge_iff_le, self_le_add_right]
     rw [hc] at hbad;
     exact (lt_irrefl c) ((ENat.add_one_le_iff c_finite).mp hbad)
-  exact h_induc (A \ B).encard A B hB hA rfl
+  exact h_induc (B \ A).encard A B hA hB rfl
 
--- this should be simp, with reversed inequality
-theorem rankMatroid_rel_rank_eq_matroid_rel_rank (M : RankMatroid α)
-    {A B : Set α} (hB : B ⊆ A) (hA : A ⊆ M.E) : M.relRank A B = M.matroid.relRank A B := by
-  obtain ⟨I, J, hJ, hI_basis_A, hJ_basis_B, h⟩ := M.matroid.rel_rank_exists hB hA
+-- drop assum, simps and swap order
+@[simp] theorem rankMatroid_relRank_eq_matroid_relRank (M : RankMatroid α)
+    {A B : Set α} : M.relRank A B = M.matroid.relRank A B := by
+  suffices h : ∀ {A B}, A ⊆ B → B ⊆ M.E → M.relRank A B = M.matroid.relRank A B by
+    set A' := A ∩ M.E
+    set B' := (B ∩ M.E) ∪ A'
+    rw [<-relRank_inter_ground, relRank_eq_union_right, <-M.matroid.relRank_inter_ground_left,
+        <-M.matroid.relRank_inter_ground_right, M.matroid.relRank_eq_union_right]
+    simp only [matroid_E]
+    refine h Set.subset_union_right ?_
+    rw [<-Set.union_inter_distrib_right]
+    exact Set.inter_subset_right
+  intro A B hA hB
+  obtain ⟨I, J, hI, ⟨hI_basis_A, _⟩, ⟨hJ_basis_B, _⟩, h⟩ := M.matroid.relRank_intro hA hB
   rw [h]; clear h;
-  unfold Matroid.Basis' maximals at hI_basis_A hJ_basis_B;
+  unfold maximals at hI_basis_A hJ_basis_B;
   simp only [matroid_Indep, Set.mem_setOf_eq, and_imp] at hI_basis_A hJ_basis_B
   obtain ⟨⟨hI_indep, hI_subset⟩, hI_max⟩ := hI_basis_A
   obtain ⟨⟨hJ_indep, hJ_subset⟩, hJ_max⟩ := hJ_basis_B
-  rw [<-M.relRank_indeps_eq_encard_diff hJ hI_indep]
-  have hAI : M.relRank A I = 0 := by
-    rw [<-indep_subset_maximal_iff_relrank_zero hA hI_subset hI_indep]
+  rw [<-M.relRank_indeps_eq_encard_diff hI hJ_indep]
+  have hIA : M.relRank I A = 0 := by
+    rw [<-indep_subset_maximal_iff_relRank_zero hI_subset hI_indep]
     unfold maximals; simp only [Set.mem_setOf_eq, and_imp]
     exact ⟨⟨hI_indep, hI_subset⟩, hI_max⟩
-  have hBJ : M.relRank B J = 0 := by
-    rw [<-indep_subset_maximal_iff_relrank_zero (hB.trans hA) hJ_subset hJ_indep]
+  have hJB : M.relRank J B = 0 := by
+    rw [<-indep_subset_maximal_iff_relRank_zero hJ_subset hJ_indep]
     unfold maximals; simp only [Set.mem_setOf_eq, and_imp]
     exact ⟨⟨hJ_indep, hJ_subset⟩, hJ_max⟩
   calc
-    M.relRank A B = M.relRank A B + M.relRank B J := by
-      rw [hBJ]; simp only [add_zero]
-    _ = M.relRank A J := by
-      exact eq_comm.mp (M.rel_rank_add_cancel hA hB hJ_subset)
-    _ = M.relRank A I + M.relRank I J := by
-      exact M.rel_rank_add_cancel hA hI_subset hJ
+    M.relRank A B = M.relRank I A + M.relRank A B := by
+      rw [hIA]; simp only [zero_add]
+    _ = M.relRank I B := by
+      exact eq_comm.mp (M.relRank_add_cancel hI_subset hA)
+    _ = M.relRank I J + M.relRank J B := by
+      exact M.relRank_add_cancel hI hJ_subset
     _ = M.relRank I J := by
-      rw [hAI]; simp only [zero_add]
+      rw [hJB]; simp only [add_zero]
 
-theorem encard_to_ncard {n : ℕ} {S : Set α} (h : S.encard = n) : S.ncard = n := by
-  have : S.Finite := by exact Set.finite_of_encard_eq_coe h
-  rw [<-Set.Finite.cast_ncard_eq this] at h
-  simp only [Nat.cast_inj] at h; assumption
+-- theorem encard_to_ncard {n : ℕ} {S : Set α} (h : S.encard = n) : S.ncard = n := by
+--   have : S.Finite := by exact Set.finite_of_encard_eq_coe h
+--   rw [<-Set.Finite.cast_ncard_eq this] at h
+--   simp only [Nat.cast_inj] at h; assumption
 
-def RankMatroid.ofFinite {E : Set α} (hE : E.Finite) (r : Set α → ℕ)
-    (rank_le_encard : ∀ (X : Set α), r X ≤ X.encard)
-    (monotonicity : {A B : Set α} → A ⊆ E → B ⊆ A → r B ≤ r A)
-    (submodularity : {A B : Set α} → A ⊆ E → B ⊆ E → (r (A ∪ B)) + (r (A ∩ B)) ≤ r A + r B)
-    : RankMatroid α where
-  E := E
-  relRank := fun A B ↦ r A - r B
-  rel_rank_le_encard_diff := by
-    intro A B hA hB; simp only [tsub_le_iff_right]
-    have hr_empty : r ∅ = 0 := by
-      have := rank_le_encard ∅
-      simp only [Set.encard_empty, nonpos_iff_eq_zero, Nat.cast_eq_zero] at this
-      assumption
-    have h := submodularity ((@Set.diff_subset α A B).trans hA) (hB.trans hA)
-    simp only [Set.diff_union_self, Set.diff_inter_self] at h
-    rw [hr_empty, Set.union_eq_self_of_subset_right hB] at h; simp only [add_zero] at h
-    have h' := rank_le_encard (A \ B)
-    have : r A ≤ (r (A \ B) + r B : ℕ∞) := by
-      rw [<-ENat.coe_add]; exact Nat.cast_le.mpr h
-    exact le_add_of_le_add_right this (rank_le_encard (A \ B))
-  rel_rank_union_le_relRank_inter := by
-    dsimp only; intro A B hA hB
-    apply Nat.mono_cast
-    simp only [Nat.cast_id]
-    apply Nat.le_sub_of_add_le
-    have : Sub.sub (r (A ∪ B)) (r B) + (r (A ∩ B)) = (r (A ∪ B)) - (r B) + (r (A ∩ B)) := by
-      exact rfl
-    rw [this, <-@Nat.sub_add_comm (r (A ∪ B)) (r (A ∩ B)) (r B) (monotonicity (Set.union_subset hA hB) (Set.subset_union_right))]
-    apply Nat.sub_le_iff_le_add.mpr
-    exact submodularity hA hB
-  rel_rank_add_cancel := by
-    intro A B C hA hB hC; dsimp only
-    refine Eq.symm (tsub_add_tsub_cancel ?hab ?hcb)
-    · exact Nat.cast_le.mpr (monotonicity hA hB)
-    exact Nat.cast_le.mpr (monotonicity (hB.trans hA) hC)
-  rel_rank_sUnion_eq_zero := by
-    dsimp only
-    intro S B hS
-    have hPE_finite : (𝒫 E).Finite := Set.Finite.finite_subsets hE
-    have hS_subset_PE : S ⊆ 𝒫 E := by
-      intro A hA; simp only [Set.mem_powerset_iff]; exact (hS A hA).2.1
-    have hS_finite : S.Finite := Set.Finite.subset hPE_finite hS_subset_PE
-    have h_induc : ∀ n : ℕ, ∀ S : Set (Set α), ∀ B, (∀ A ∈ S, B ⊆ A ∧ A ⊆ E ∧ (r A : ℕ∞) - (r B : ℕ∞) = 0) → S.encard = n → r (⋃₀ S) - r B = 0 := by
-      intro n
-      induction n with
-      | zero =>
-        intro S B hS hS_encard
-        have : ⋃₀ S = ∅ := by
-          rw [<-Set.sUnion_empty]
-          refine congrArg Set.sUnion ?_
-          exact Set.encard_eq_zero.mp hS_encard
-        have h : r ∅ = 0 := by
-          have := (rank_le_encard ∅)
-          simp only [Set.encard_empty, nonpos_iff_eq_zero, Nat.cast_eq_zero] at this
-          assumption
-        rw [this, h]; simp only [ge_iff_le, zero_le, tsub_eq_zero_of_le]
-      | succ n hn =>
-        intro S B hS hS_encard
-        have hS_rank : ∀ A ∈ S, r A = r B := by
-          intro A hA
-          have h₁ := (hS A hA).2.2
-          have h₂ := monotonicity (hS A hA).2.1 (hS A hA).1
-          rw [<-ENat.coe_sub] at h₁
-          have : r A - r B = 0 := by exact WithTop.coe_eq_zero.mp h₁
-          have := (Nat.sub_eq_iff_eq_add h₂).mp this
-          simp only [zero_add] at this; assumption
-        obtain ⟨A, S₀, ⟨h_nmem, h_ins, h_ncard⟩⟩ := Set.eq_insert_of_ncard_eq_succ (encard_to_ncard hS_encard)
-        rw [<-h_ins] at hS_rank hS hS_encard ⊢
-        rw [Set.sUnion_insert A S₀]
-        have hS₀_subsetE : ⋃₀ S₀ ⊆ E := by
-          apply Set.sUnion_subset_iff.mpr
-          intro B hB; exact (hS B (Set.mem_insert_of_mem A hB)).2.1
-        have hB_subsetS₀ : B ⊆ ⋃₀ S₀ := by
-          sorry
-        have h : r (A ∪ ⋃₀ S₀) + r (A ∩ ⋃₀ S₀) ≤ r A + r (⋃₀ S₀) := by
-          exact submodularity (hS A (Set.mem_insert A S₀)).2.1 hS₀_subsetE
-        have hS₀_encard : S₀.encard = n := by
-          rw [Set.encard_insert_of_not_mem h_nmem] at hS_encard
-          simp only [Nat.cast_add, Nat.cast_one] at hS_encard
-          sorry
-        simp only [Set.sUnion_insert] at hn
-        have hS₀ : (∀ A ∈ S₀, B ⊆ A ∧ A ⊆ E ∧ (r A : ℕ∞) - r B = 0) := by
-          intro A' hA'; exact hS A' (Set.mem_insert_of_mem A hA')
-        have : r (⋃₀ S₀) = r B := by
-          have := hn S₀ B hS₀ hS₀_encard
-          rw [Nat.sub_eq_iff_eq_add (monotonicity hS₀_subsetE hB_subsetS₀)] at this
-          simp only [zero_add] at this; assumption
-        rw [this, hS_rank A (Set.mem_insert A S₀)] at h
-        have : r (A ∩ ⋃₀ S₀) = r B := by
-          apply le_antisymm_iff.mpr; constructor
-          · rw [<-this]; exact monotonicity hS₀_subsetE (Set.inter_subset_right)
-          exact monotonicity (Set.inter_subset_right.trans hS₀_subsetE) (Set.subset_inter (hS A (Set.mem_insert A S₀)).1 hB_subsetS₀)
-        rw [this] at h; simp only [add_le_add_iff_right] at h
-        exact Nat.sub_eq_zero_of_le h
-    have := h_induc (ENat.toNat S.encard) S B hS (eq_comm.mp (ENat.coe_toNat_eq_self.mpr (Set.encard_ne_top_iff.mpr hS_finite)))
-    exact @congrArg ℕ ℕ∞ (r (⋃₀ S) - r B) 0 Nat.cast this
+-- def ofFinite {E : Set α} (hE : E.Finite) (r : Set α → ℕ)
+--     (rank_le_encard : ∀ (X : Set α), r X ≤ X.encard)
+--     (monotonicity : {A B : Set α} → A ⊆ E → B ⊆ A → r B ≤ r A)
+--     (submodularity : {A B : Set α} → A ⊆ E → B ⊆ E → (r (A ∪ B)) + (r (A ∩ B)) ≤ r A + r B)
+--     : RankMatroid α where
+--   E := E
+--   relRank := fun A B ↦ r A - r B
+--   relRank_le_encard_diff := by
+--     intro A B hA hB; simp only [tsub_le_iff_right]
+--     have hr_empty : r ∅ = 0 := by
+--       have := rank_le_encard ∅
+--       simp only [Set.encard_empty, nonpos_iff_eq_zero, Nat.cast_eq_zero] at this
+--       assumption
+--     have h := submodularity ((@Set.diff_subset α A B).trans hA) (hB.trans hA)
+--     simp only [Set.diff_union_self, Set.diff_inter_self] at h
+--     rw [hr_empty, Set.union_eq_self_of_subset_right hB] at h; simp only [add_zero] at h
+--     have h' := rank_le_encard (A \ B)
+--     have : r A ≤ (r (A \ B) + r B : ℕ∞) := by
+--       rw [<-ENat.coe_add]; exact Nat.cast_le.mpr h
+--     exact le_add_of_le_add_right this (rank_le_encard (A \ B))
+--   relRank_union_le_relRank_inter := by
+--     dsimp only; intro A B hA hB
+--     apply Nat.mono_cast
+--     simp only [Nat.cast_id]
+--     apply Nat.le_sub_of_add_le
+--     have : Sub.sub (r (A ∪ B)) (r B) + (r (A ∩ B)) = (r (A ∪ B)) - (r B) + (r (A ∩ B)) := by
+--       exact rfl
+--     rw [this, <-@Nat.sub_add_comm (r (A ∪ B)) (r (A ∩ B)) (r B) (monotonicity (Set.union_subset hA hB) (Set.subset_union_right))]
+--     apply Nat.sub_le_iff_le_add.mpr
+--     exact submodularity hA hB
+--   relRank_add_cancel := by
+--     intro A B C hA hB hC; dsimp only
+--     refine Eq.symm (tsub_add_tsub_cancel ?hab ?hcb)
+--     · exact Nat.cast_le.mpr (monotonicity hA hB)
+--     exact Nat.cast_le.mpr (monotonicity (hB.trans hA) hC)
+--   relRank_sUnion_eq_zero := by
+--     dsimp only
+--     intro S B hS
+--     have hPE_finite : (𝒫 E).Finite := Set.Finite.finite_subsets hE
+--     have hS_subset_PE : S ⊆ 𝒫 E := by
+--       intro A hA; simp only [Set.mem_powerset_iff]; exact (hS A hA).2.1
+--     have hS_finite : S.Finite := Set.Finite.subset hPE_finite hS_subset_PE
+--     have h_induc : ∀ n : ℕ, ∀ S : Set (Set α), ∀ B, (∀ A ∈ S, B ⊆ A ∧ A ⊆ E ∧ (r A : ℕ∞) - (r B : ℕ∞) = 0) → S.encard = n → r (⋃₀ S) - r B = 0 := by
+--       intro n
+--       induction n with
+--       | zero =>
+--         intro S B hS hS_encard
+--         have : ⋃₀ S = ∅ := by
+--           rw [<-Set.sUnion_empty]
+--           refine congrArg Set.sUnion ?_
+--           exact Set.encard_eq_zero.mp hS_encard
+--         have h : r ∅ = 0 := by
+--           have := (rank_le_encard ∅)
+--           simp only [Set.encard_empty, nonpos_iff_eq_zero, Nat.cast_eq_zero] at this
+--           assumption
+--         rw [this, h]; simp only [ge_iff_le, zero_le, tsub_eq_zero_of_le]
+--       | succ n hn =>
+--         intro S B hS hS_encard
+--         have hS_rank : ∀ A ∈ S, r A = r B := by
+--           intro A hA
+--           have h₁ := (hS A hA).2.2
+--           have h₂ := monotonicity (hS A hA).2.1 (hS A hA).1
+--           rw [<-ENat.coe_sub] at h₁
+--           have : r A - r B = 0 := by exact WithTop.coe_eq_zero.mp h₁
+--           have := (Nat.sub_eq_iff_eq_add h₂).mp this
+--           simp only [zero_add] at this; assumption
+--         obtain ⟨A, S₀, ⟨h_nmem, h_ins, h_ncard⟩⟩ := Set.eq_insert_of_ncard_eq_succ (encard_to_ncard hS_encard)
+--         rw [<-h_ins] at hS_rank hS hS_encard ⊢
+--         rw [Set.sUnion_insert A S₀]
+--         have hS₀_subsetE : ⋃₀ S₀ ⊆ E := by
+--           apply Set.sUnion_subset_iff.mpr
+--           intro B hB; exact (hS B (Set.mem_insert_of_mem A hB)).2.1
+--         have hB_subsetS₀ : B ⊆ ⋃₀ S₀ := by
+--           sorry
+--         have h : r (A ∪ ⋃₀ S₀) + r (A ∩ ⋃₀ S₀) ≤ r A + r (⋃₀ S₀) := by
+--           exact submodularity (hS A (Set.mem_insert A S₀)).2.1 hS₀_subsetE
+--         have hS₀_encard : S₀.encard = n := by
+--           rw [Set.encard_insert_of_not_mem h_nmem] at hS_encard
+--           simp only [Nat.cast_add, Nat.cast_one] at hS_encard
+--           sorry
+--         simp only [Set.sUnion_insert] at hn
+--         have hS₀ : (∀ A ∈ S₀, B ⊆ A ∧ A ⊆ E ∧ (r A : ℕ∞) - r B = 0) := by
+--           intro A' hA'; exact hS A' (Set.mem_insert_of_mem A hA')
+--         have : r (⋃₀ S₀) = r B := by
+--           have := hn S₀ B hS₀ hS₀_encard
+--           rw [Nat.sub_eq_iff_eq_add (monotonicity hS₀_subsetE hB_subsetS₀)] at this
+--           simp only [zero_add] at this; assumption
+--         rw [this, hS_rank A (Set.mem_insert A S₀)] at h
+--         have : r (A ∩ ⋃₀ S₀) = r B := by
+--           apply le_antisymm_iff.mpr; constructor
+--           · rw [<-this]; exact monotonicity hS₀_subsetE (Set.inter_subset_right)
+--           exact monotonicity (Set.inter_subset_right.trans hS₀_subsetE) (Set.subset_inter (hS A (Set.mem_insert A S₀)).1 hB_subsetS₀)
+--         rw [this] at h; simp only [add_le_add_iff_right] at h
+--         exact Nat.sub_eq_zero_of_le h
+--     have := h_induc (ENat.toNat S.encard) S B hS (eq_comm.mp (ENat.coe_toNat_eq_self.mpr (Set.encard_ne_top_iff.mpr hS_finite)))
+--     exact @congrArg ℕ ℕ∞ (r (⋃₀ S) - r B) 0 Nat.cast this
 
-  Indep := fun X ↦ X ⊆ E ∧ r X = X.encard
-  indep_maximal := by
-    intro X hX I hI hI'; dsimp only
-    set S := {Y | (Y ⊆ E ∧ ↑(r Y) = Y.encard) ∧ I ⊆ Y ∧ Y ⊆ X}
-    have : S ⊆ 𝒫 X := fun Y hY ↦ hY.2.2
-    have : S.Finite := by
-      exact Set.Finite.subset (Set.Finite.finite_subsets (Set.Finite.subset hE hX)) this
-    unfold maximals Set.Nonempty
-    have hS_nonempty : S.Nonempty := by
-      unfold Set.Nonempty; use I
-      exact ⟨⟨hI'.trans hX, hI.2⟩, subset_refl I, hI'⟩
-    rcases Set.Finite.exists_maximal_wrt (fun A ↦ A) S this hS_nonempty with ⟨M, hMS, hM_max⟩
-    use M; dsimp only [Set.sep_setOf, Set.mem_setOf_eq]
-    refine ⟨hMS, ?_⟩
-    intro M' hM'S hM'
-    rw [hM_max M' hM'S hM']
-  indep_iff' := by
-    simp only [gt_iff_lt, tsub_pos_iff_lt, Nat.cast_lt]
-    refine fun I ↦ ⟨fun ⟨hI_subset, hIr⟩ ↦ ⟨hI_subset, ?_⟩, fun ⟨hI_subset, hI⟩ ↦ ⟨hI_subset, ?_⟩⟩
-    · intro x hx
-      have hIr := encard_to_ncard (Eq.symm hIr)
-      have hI_finite : I.Finite := by exact Set.Finite.subset hE hI_subset
-      have : r (I \ {x}) ≤ r I - 1 := by
-        rw [<-hIr, <-Set.ncard_diff_singleton_of_mem hx hI_finite]
-        have := rank_le_encard (I \ {x})
-        rw [<-Set.Finite.cast_ncard_eq (Set.Finite.subset hI_finite Set.diff_subset)] at this
-        exact WithTop.coe_le_coe.mp this
-      have hrI : r I > 0 := by
-        rw [<-hIr]; exact Nat.zero_lt_of_ne_zero (Set.ncard_ne_zero_of_mem hx hI_finite)
-      exact (Nat.lt_iff_le_pred hrI).mpr this
-    sorry
+--   Indep := fun X ↦ X ⊆ E ∧ r X = X.encard
+--   indep_maximal := by
+--     intro X hX I hI hI'; dsimp only
+--     set S := {Y | (Y ⊆ E ∧ ↑(r Y) = Y.encard) ∧ I ⊆ Y ∧ Y ⊆ X}
+--     have : S ⊆ 𝒫 X := fun Y hY ↦ hY.2.2
+--     have : S.Finite := by
+--       exact Set.Finite.subset (Set.Finite.finite_subsets (Set.Finite.subset hE hX)) this
+--     unfold maximals Set.Nonempty
+--     have hS_nonempty : S.Nonempty := by
+--       unfold Set.Nonempty; use I
+--       exact ⟨⟨hI'.trans hX, hI.2⟩, subset_refl I, hI'⟩
+--     rcases Set.Finite.exists_maximal_wrt (fun A ↦ A) S this hS_nonempty with ⟨M, hMS, hM_max⟩
+--     use M; dsimp only [Set.sep_setOf, Set.mem_setOf_eq]
+--     refine ⟨hMS, ?_⟩
+--     intro M' hM'S hM'
+--     rw [hM_max M' hM'S hM']
+--   indep_iff' := by
+--     simp only [gt_iff_lt, tsub_pos_iff_lt, Nat.cast_lt]
+--     refine fun I ↦ ⟨fun ⟨hI_subset, hIr⟩ ↦ ⟨hI_subset, ?_⟩, fun ⟨hI_subset, hI⟩ ↦ ⟨hI_subset, ?_⟩⟩
+--     · intro x hx
+--       have hIr := encard_to_ncard (Eq.symm hIr)
+--       have hI_finite : I.Finite := by exact Set.Finite.subset hE hI_subset
+--       have : r (I \ {x}) ≤ r I - 1 := by
+--         rw [<-hIr, <-Set.ncard_diff_singleton_of_mem hx hI_finite]
+--         have := rank_le_encard (I \ {x})
+--         rw [<-Set.Finite.cast_ncard_eq (Set.Finite.subset hI_finite Set.diff_subset)] at this
+--         exact WithTop.coe_le_coe.mp this
+--       have hrI : r I > 0 := by
+--         rw [<-hIr]; exact Nat.zero_lt_of_ne_zero (Set.ncard_ne_zero_of_mem hx hI_finite)
+--       exact (Nat.lt_iff_le_pred hrI).mpr this
+--     sorry
 end RankMatroid
